deps/poulet4/lib/P4automata/Bisimulations.v
@@ -903,13 +903,194 @@ Module SynPreSynWP1bit.
                     |intuition].
     Qed.
 
-    Lemma wp_op:
-      forall c (valu: bval c) o phi s1 st1 buf1 c2,
+    Lemma wp_op'_size:
+      forall (c: bctx) si o n phi m phi',
+        WP.wp_op' (c:=c) si o (P4A.op_size o + n, phi) = (m, phi') ->
+        m = n.
+    Proof.
+      induction o; cbn; intros.
+      - congruence.
+      - destruct (WP.wp_op' si o2 (P4A.op_size o1 + P4A.op_size o2 + n, phi)) eqn:?.
+        replace (P4A.op_size o1 + P4A.op_size o2 + n)
+          with (P4A.op_size o2 + (P4A.op_size o1 + n))
+          in *
+          by Lia.lia.
+        apply IHo2 in Heqp.
+        subst.
+        eauto.
+      - replace (width + n - width) with n in * by Lia.lia.
+        congruence.
+      - congruence.
+    Qed.
+
+    Lemma wp_op'_seq:
+      forall (c: bctx) o1 o2 si phi,
+        WP.wp_op' (c:=c) si (P4A.OpSeq o1 o2) phi = WP.wp_op' si o1 (WP.wp_op' si o2 phi).
+    Proof.
+      induction o1; intros; simpl;
+        repeat match goal with
+               | H:context [match ?x with _ => _ end] |- _ => destruct x eqn:?; simpl
+               | |- context [match ?x with _ => _ end] => destruct x eqn:?; simpl
+               | H: (_, _) = (_, _) |- _ => inversion H; clear H; subst
+               end.
+      - reflexivity.
+      - rewrite <- IHo1_1.
+        reflexivity.
+      - reflexivity.
+      - reflexivity.
+    Qed.
+
+    Ltac break_match :=
+      match goal with
+      | |- context [match ?x with _ => _ end] =>
+        destruct x eqn:?
+      | H: context [match ?x with _ => _ end] |- _ =>
+        destruct x eqn:?
+      end.
+
+    Lemma skipn_skipn:
+      forall A (l: list A) m n,
+        skipn n (skipn m l) = skipn (n + m) l.
+    Proof.
+      induction l; intros.
+      - rewrite !skipn_nil.
+        reflexivity.
+      - destruct m.
+        + simpl.
+          rewrite <- plus_n_O.
+          reflexivity.
+        + rewrite skipn_cons.
+          replace (n + S m) with (S (n + m))
+            by eauto with *.
+          rewrite skipn_cons.
+          eauto.
+    Qed.
+
+    Lemma eval_op_buf_skip:
+      forall st buf o st' buf',
+        P4A.eval_op st buf o = (st', buf') ->
+        exists m,
+          buf' = skipn m buf.
+    Proof.
+      intros.
+      replace buf' with (snd (P4A.eval_op st buf o))
+        by (rewrite H0; reflexivity).
+      replace st' with (fst (P4A.eval_op st buf o))
+        by (rewrite H0; reflexivity).
+      clear H0.
+      clear buf'.
+      clear st'.
+      revert st.
+      revert buf.
+      induction o; cbn in *; intros.
+      - exists 0.
+        reflexivity.
+      - destruct (IHo1 buf st) as [m1 IHo1'].
+        break_match; simpl in *; subst.
+        destruct (IHo2 (skipn m1 buf) s) as [m2 IHo2'].
+        exists (m1 + m2).
+        rewrite IHo2'.
+        rewrite skipn_skipn.
+        rewrite Plus.plus_comm.
+        reflexivity.
+      - exists width.
+        reflexivity.
+      - exists 0.
+        reflexivity.
+    Qed.
+
+    Lemma wp_op'_mono:
+      forall (c: bctx) si o n phi,
+        fst (WP.wp_op' (c:=c) si o (n, phi)) <= n.
+    Proof.
+      induction o; simpl.
+      - Lia.lia.
+      - intros.
+        destruct (WP.wp_op' si o2 _) as [m psi] eqn:?.
+        specialize (IHo2 n phi).
+        specialize (IHo1 m psi).
+        rewrite Heqp in *.
+        simpl in *.
+        Lia.lia.
+      - Lia.lia.
+      - Lia.lia.
+    Qed.
+
+    Lemma eval_op_list:
+      forall o st buf st' buf',
+        P4A.eval_op st buf o = (st', buf') ->
+        List.length buf >= P4A.op_size o ->
+        exists chunk,
+          length chunk = P4A.op_size o /\
+          chunk ++ buf' = buf.
+    Proof.
+      induction o; intros; simpl in *.
+      - exists nil.
+        simpl.
+        split; congruence.
+      - destruct (P4A.eval_op st buf o1) as [st1 buf1] eqn:?.
+        destruct (P4A.eval_op st1 buf1 o2) as [st2 buf2] eqn:?.
+        inversion H0; subst; clear H0.
+        destruct (IHo1 st buf st1 buf1 ltac:(auto) ltac:(Lia.lia)) as [chunk1 [Hlen1 Hc1]].
+        destruct (IHo2 st1 buf1 st' buf' ltac:(auto)) as [chunk2 [Hlen2 Hc2]].
+        {
+          pose proof (f_equal (@List.length bool) Hc1).
+          rewrite app_length in *.
+          Lia.lia.
+        }
+        subst.
+        exists (chunk1 ++ chunk2).
+        split.
+        + rewrite app_length.
+          congruence.
+        + rewrite <- app_assoc.
+          congruence.
+      - exists (firstn width buf).
+        split.
+        + apply firstn_length_le.
+          Lia.lia.
+        + inversion H0.
+          apply firstn_skipn.
+      - exists nil.
+        inversion H0.
+        auto.
+    Qed.
+
+    Lemma eval_op_size:
+      forall o st buf,
+        length (snd (P4A.eval_op st buf o)) = length buf - P4A.op_size o.
+    Proof.
+      induction o; intros; simpl.
+      - simpl.
+        Lia.lia.
+      - destruct (P4A.eval_op st buf o1) as [st' buf'] eqn:?.
+        destruct (P4A.eval_op st' buf' o2) as [st'' buf''] eqn:?.
+        specialize (IHo1 st buf).
+        rewrite Heqp in IHo1.
+        specialize (IHo2 st' buf').
+        rewrite Heqp0 in IHo2.
+        simpl in *.
+        Lia.lia.
+      - exact (skipn_length width buf).
+      - Lia.lia.
+    Qed.
+
+    Lemma expr_to_bit_expr_sound:
+      forall (c: bctx) si (valu: bval c) expr c1 c2,
+        P4A.eval_expr (snd (fst match si with Left => c1 | Right => c2 end)) expr = P4A.VBits (interp_bit_expr (a:=a) (WP.expr_to_bit_expr si expr) valu c1 c2).
+    Proof.
+    Admitted.
+
+    Notation "⟨ R , v ⟩ ⊨ c1 c2" := (interp_store_rel R v c1 c2) (at level 50).
+    Lemma wp_op'_spec:
+      forall c (valu: bval c) o n phi s1 st1 buf1 c2,
+        length buf1 = n + P4A.op_size o ->
+        (forall width h, o = P4A.OpExtract width h -> width > 0) ->
         interp_store_rel (a:=a)
-                         (WP.wp_op Left o phi)
+                         (snd (WP.wp_op' Left o (P4A.op_size o, phi)))
                          valu
                          (s1, st1, buf1)
-                         c2 ->
+                         c2 <->
         interp_store_rel (a:=a)
                          phi
                          valu
@@ -919,19 +1100,97 @@ Module SynPreSynWP1bit.
                          c2.
     Proof.
       induction o.
-      - cbn; tauto.
-      - admit.
-      - unfold WP.wp_op, WP.wp_op'.
+      - intros.
+        simpl.
+        reflexivity.
+      - intros.
+        simpl (P4A.eval_op _ _ _).
+        destruct (P4A.eval_op st1 (skipn (P4A.op_size o1 + P4A.op_size o2) buf1) o1) as [st1' buf1'] eqn:?.
+        destruct (P4A.eval_op st1' buf1' o2) as [st2' buf2'] eqn:?.
+        (*
+        assert (length buf1' = length buf1 - P4A.op_size o1).
+        {
+          replace buf1'
+            with (snd (P4A.eval_op st1 buf1 o1))
+            by (rewrite Heqp; reflexivity).
+          eapply eval_op_size.
+        }
+        assert (length buf2' = length buf1' - P4A.op_size o2).
+        {
+          replace buf2'
+            with (snd (P4A.eval_op st1' buf1' o2))
+            by (rewrite Heqp0; reflexivity).
+          eapply eval_op_size.
+        }
+        simpl in H0.
+        destruct (eval_op_list _ _ _ _ _ Heqp ltac:(Lia.lia)) as [chunk1 [Hlen1 Hc1]].
+        destruct (eval_op_list _ _ _ _ _ Heqp0 ltac:(Lia.lia)) as [chunk2 [Hlen2 Hc2]].
+        subst.
+        rewrite !app_length, Plus.plus_assoc in *.
+        cbn in *.
+        destruct (WP.wp_op' Left o2 (P4A.op_size o1 + P4A.op_size o2 + n, phi)) as [n' phi'] eqn:?.
+        assert (n' = P4A.op_size o1 + n).
+        {
+          replace (P4A.op_size o1 + P4A.op_size o2 + n)
+            with (P4A.op_size o2 + (P4A.op_size o1 + n))
+            in Heqp1
+            by Lia.lia.
+          eapply wp_op'_size.
+          eauto.
+        }
+        destruct (WP.wp_op' Left o1 (n', phi')) as [n'' phi''] eqn:?.
+        assert (n'' = n).
+        {
+          subst n'.
+          eapply wp_op'_size.
+          eauto.
+        }
+        subst n''.
+        assert (length buf2' >= n) by Lia.lia.
+        replace (n + (P4A.op_size o1 + P4A.op_size o2))
+          with (P4A.op_size o1 + P4A.op_size o2 + n)
+          by Lia.lia.
+        rewrite Heqp1.
+        subst n'.
+        rewrite (Plus.plus_comm _ n).
+        erewrite IHo1 by (rewrite !app_length in *; Lia.lia).
+        replace (s1, st2', buf2')
+          with (s1,
+                fst (P4A.eval_op st1' (chunk2 ++ buf2') o2),
+                snd (P4A.eval_op st1' (chunk2 ++ buf2') o2))
+          by (rewrite Heqp0; reflexivity).
+        erewrite <- (IHo2 n)
+          by (rewrite !app_length in *; Lia.lia).
+        rewrite !Heqp; simpl.
+        Morphisms.f_equiv.
+        replace phi' with (snd (WP.wp_op' Left o2 (P4A.op_size o1 + P4A.op_size o2 + n, phi)))
+          by (rewrite Heqp1; reflexivity).
+         *)
+        admit.
+      - simpl.
+        unfold WP.wp_op, WP.wp_op'.
         simpl.
         intros.
-        induction phi; simpl; intros.
-        + tauto.
-        + tauto.
-        + admit.
-        + admit.
-        + admit.
-        + admit.
-      - admit.
+        rewrite sr_subst_hdr_left.
+        simpl.
+        replace (width - width) with 0 by Lia.lia.
+        simpl.
+        unfold P4A.slice.
+        specialize (H1 _ _ ltac:(eauto)).
+        replace (1 + (width - 1)) with width by Lia.lia.
+        rewrite skipn_O.
+        Morphisms.f_equiv.
+        f_equal.
+        admit.
+      - simpl.
+        unfold WP.wp_op, WP.wp_op'.
+        simpl.
+        intros.
+        destruct lhs.
+        rewrite sr_subst_hdr_left.
+        simpl.
+        rewrite <- expr_to_bit_expr_sound.
+        reflexivity.
     Admitted.
 
     Lemma wp_pred_pair_step :
